tests/elab/grind_ematch_diag_2.lean
@@ -303,9 +303,9 @@ h_7 : idx + 8 ≤ len
     [thm] Excessively Branching Instances
       [thm] next_def: next (slot s (idx + 1)) = slot s (idx + 1 + 1) has 16 direct follow up instances
         [thm] sorted: idx + 2 < len → lookup heap (slot s (idx + 2)) ≤ lookup heap (next (slot s (idx + 2)))
-        [thm] inj: idx + 2 ≠ idx + 7 → slot s (idx + 2) ≠ slot s (idx + 7)
         [thm] inj: idx + 2 ≠ idx + 5 → slot s (idx + 2) ≠ slot s (idx + 5)
         [thm] inj: idx ≠ idx + 2 → slot s idx ≠ slot s (idx + 2)
+        [thm] inj: idx + 2 ≠ idx + 7 → slot s (idx + 2) ≠ slot s (idx + 7)
         [thm] inj: idx + 6 ≠ idx + 2 → slot s (idx + 6) ≠ slot s (idx + 2)
         [thm] inj: idx + 1 ≠ idx + 2 → slot s (idx + 1) ≠ slot s (idx + 2)
         [thm] inj: idx + 2 ≠ idx + 6 → slot s (idx + 2) ≠ slot s (idx + 6)
@@ -326,15 +326,15 @@ h_7 : idx + 8 ≤ len
         [thm] inj: idx + 3 ≠ idx → slot s (idx + 3) ≠ slot s idx
         [thm] sorted: idx + 3 < len → lookup heap (slot s (idx + 3)) ≤ lookup heap (next (slot s (idx + 3)))
         [thm] inj: idx ≠ idx + 3 → slot s idx ≠ slot s (idx + 3)
-        [thm] inj: idx + 5 ≠ idx + 3 → slot s (idx + 5) ≠ slot s (idx + 3)
-        [thm] inj: idx + 3 ≠ idx + 6 → slot s (idx + 3) ≠ slot s (idx + 6)
         [thm] inj: idx + 3 ≠ idx + 1 → slot s (idx + 3) ≠ slot s (idx + 1)
+        [thm] inj: idx + 5 ≠ idx + 3 → slot s (idx + 5) ≠ slot s (idx + 3)
         [thm] inj: idx + 2 ≠ idx + 3 → slot s (idx + 2) ≠ slot s (idx + 3)
         [thm] inj: idx + 6 ≠ idx + 3 → slot s (idx + 6) ≠ slot s (idx + 3)
+        [thm] inj: idx + 3 ≠ idx + 6 → slot s (idx + 3) ≠ slot s (idx + 6)
         [thm] inj: idx + 3 ≠ idx + 2 → slot s (idx + 3) ≠ slot s (idx + 2)
         [thm] inj: idx + 7 ≠ idx + 3 → slot s (idx + 7) ≠ slot s (idx + 3)
-        [thm] inj: idx + 3 ≠ idx + 7 → slot s (idx + 3) ≠ slot s (idx + 7)
         [thm] inj: idx + 3 ≠ idx + 4 → slot s (idx + 3) ≠ slot s (idx + 4)
+        [thm] inj: idx + 3 ≠ idx + 7 → slot s (idx + 3) ≠ slot s (idx + 7)
       [thm] next_def: next (slot s (idx + 3)) = slot s (idx + 3 + 1) has 16 direct follow up instances
         [thm] inj: idx + 4 ≠ idx + 1 → slot s (idx + 4) ≠ slot s (idx + 1)
         [thm] sorted: idx + 4 < len → lookup heap (slot s (idx + 4)) ≤ lookup heap (next (slot s (idx + 4)))
@@ -347,12 +347,13 @@ h_7 : idx + 8 ≤ len
         [thm] inj: idx + 7 ≠ idx + 4 → slot s (idx + 7) ≠ slot s (idx + 4)
         [thm] inj: idx + 4 ≠ idx + 5 → slot s (idx + 4) ≠ slot s (idx + 5)
         [thm] inj: idx + 2 ≠ idx + 4 → slot s (idx + 2) ≠ slot s (idx + 4)
-        [thm] inj: idx + 4 ≠ idx + 7 → slot s (idx + 4) ≠ slot s (idx + 7)
         [thm] inj: idx + 6 ≠ idx + 4 → slot s (idx + 6) ≠ slot s (idx + 4)
+        [thm] inj: idx + 4 ≠ idx + 7 → slot s (idx + 4) ≠ slot s (idx + 7)
         [thm] inj: idx + 4 ≠ idx + 6 → slot s (idx + 4) ≠ slot s (idx + 6)
         [thm] inj: idx + 3 ≠ idx + 4 → slot s (idx + 3) ≠ slot s (idx + 4)
         [thm] inj: idx + 4 ≠ idx + 2 → slot s (idx + 4) ≠ slot s (idx + 2)
       [thm] next_def: next (slot s (idx + 4)) = slot s (idx + 4 + 1) has 16 direct follow up instances
+        [thm] inj: idx + 6 ≠ idx + 5 → slot s (idx + 6) ≠ slot s (idx + 5)
         [thm] inj: idx + 2 ≠ idx + 5 → slot s (idx + 2) ≠ slot s (idx + 5)
         [thm] inj: idx + 3 ≠ idx + 5 → slot s (idx + 3) ≠ slot s (idx + 5)
         [thm] inj: idx + 5 ≠ idx + 4 → slot s (idx + 5) ≠ slot s (idx + 4)
@@ -360,22 +361,21 @@ h_7 : idx + 8 ≤ len
         [thm] inj: idx + 5 ≠ idx + 1 → slot s (idx + 5) ≠ slot s (idx + 1)
         [thm] inj: idx + 1 ≠ idx + 5 → slot s (idx + 1) ≠ slot s (idx + 5)
         [thm] inj: idx + 5 ≠ idx + 7 → slot s (idx + 5) ≠ slot s (idx + 7)
-        [thm] inj: idx + 5 ≠ idx + 6 → slot s (idx + 5) ≠ slot s (idx + 6)
         [thm] next_def: next (slot s (idx + 5)) = slot s (idx + 5 + 1)
         [thm] inj: idx + 4 ≠ idx + 5 → slot s (idx + 4) ≠ slot s (idx + 5)
+        [thm] inj: idx + 5 ≠ idx + 6 → slot s (idx + 5) ≠ slot s (idx + 6)
         [thm] inj: idx + 5 ≠ idx + 3 → slot s (idx + 5) ≠ slot s (idx + 3)
         [thm] inj: idx + 5 ≠ idx + 2 → slot s (idx + 5) ≠ slot s (idx + 2)
         [thm] inj: idx ≠ idx + 5 → slot s idx ≠ slot s (idx + 5)
         [thm] sorted: idx + 5 < len → lookup heap (slot s (idx + 5)) ≤ lookup heap (next (slot s (idx + 5)))
         [thm] inj: idx + 5 ≠ idx → slot s (idx + 5) ≠ slot s idx
-        [thm] inj: idx + 6 ≠ idx + 5 → slot s (idx + 6) ≠ slot s (idx + 5)
       [thm] next_def: next (slot s (idx + 5)) = slot s (idx + 5 + 1) has 16 direct follow up instances
         [thm] inj: idx + 7 ≠ idx + 6 → slot s (idx + 7) ≠ slot s (idx + 6)
         [thm] inj: idx + 6 ≠ idx + 2 → slot s (idx + 6) ≠ slot s (idx + 2)
-        [thm] inj: idx + 6 ≠ idx + 7 → slot s (idx + 6) ≠ slot s (idx + 7)
         [thm] inj: idx + 6 ≠ idx + 1 → slot s (idx + 6) ≠ slot s (idx + 1)
         [thm] inj: idx ≠ idx + 6 → slot s idx ≠ slot s (idx + 6)
         [thm] inj: idx + 2 ≠ idx + 6 → slot s (idx + 2) ≠ slot s (idx + 6)
+        [thm] inj: idx + 6 ≠ idx + 7 → slot s (idx + 6) ≠ slot s (idx + 7)
         [thm] sorted: idx + 6 < len → lookup heap (slot s (idx + 6)) ≤ lookup heap (next (slot s (idx + 6)))
         [thm] inj: idx + 6 ≠ idx → slot s (idx + 6) ≠ slot s idx
         [thm] next_def: next (slot s (idx + 6)) = slot s (idx + 6 + 1)
@@ -394,8 +394,8 @@ h_7 : idx + 8 ≤ len
         [thm] inj: idx + 1 ≠ idx + 7 → slot s (idx + 1) ≠ slot s (idx + 7)
         [thm] inj: idx + 6 ≠ idx + 7 → slot s (idx + 6) ≠ slot s (idx + 7)
         [thm] next_def: next (slot s (idx + 7)) = slot s (idx + 7 + 1)
-        [thm] inj: idx + 5 ≠ idx + 7 → slot s (idx + 5) ≠ slot s (idx + 7)
         [thm] inj: idx + 7 ≠ idx + 4 → slot s (idx + 7) ≠ slot s (idx + 4)
+        [thm] inj: idx + 5 ≠ idx + 7 → slot s (idx + 5) ≠ slot s (idx + 7)
         [thm] inj: idx + 7 ≠ idx → slot s (idx + 7) ≠ slot s idx
         [thm] inj: idx + 4 ≠ idx + 7 → slot s (idx + 4) ≠ slot s (idx + 7)
         [thm] inj: idx + 7 ≠ idx + 2 → slot s (idx + 7) ≠ slot s (idx + 2)
@@ -405,13 +405,13 @@ h_7 : idx + 8 ≤ len
         [thm] inj: idx + 3 ≠ idx + 7 → slot s (idx + 3) ≠ slot s (idx + 7)
       [thm] next_def: next (slot s idx) = slot s (idx + 1) has 15 direct follow up instances
         [thm] inj: idx + 4 ≠ idx + 1 → slot s (idx + 4) ≠ slot s (idx + 1)
-        [thm] inj: idx + 1 ≠ idx + 7 → slot s (idx + 1) ≠ slot s (idx + 7)
         [thm] inj: idx + 1 ≠ idx + 2 → slot s (idx + 1) ≠ slot s (idx + 2)
         [thm] inj: idx + 5 ≠ idx + 1 → slot s (idx + 5) ≠ slot s (idx + 1)
-        [thm] inj: idx + 6 ≠ idx + 1 → slot s (idx + 6) ≠ slot s (idx + 1)
         [thm] inj: idx + 1 ≠ idx + 4 → slot s (idx + 1) ≠ slot s (idx + 4)
         [thm] inj: idx + 1 ≠ idx + 5 → slot s (idx + 1) ≠ slot s (idx + 5)
+        [thm] inj: idx + 6 ≠ idx + 1 → slot s (idx + 6) ≠ slot s (idx + 1)
         [thm] inj: idx + 1 ≠ idx + 3 → slot s (idx + 1) ≠ slot s (idx + 3)
+        [thm] inj: idx + 1 ≠ idx + 7 → slot s (idx + 1) ≠ slot s (idx + 7)
         [thm] next_def: next (slot s (idx + 1)) = slot s (idx + 1 + 1)
         [thm] inj: idx ≠ idx + 1 → slot s idx ≠ slot s (idx + 1)
         [thm] inj: idx + 2 ≠ idx + 1 → slot s (idx + 2) ≠ slot s (idx + 1)
@@ -419,6 +419,7 @@ h_7 : idx + 8 ≤ len
         [thm] inj: idx + 1 ≠ idx + 6 → slot s (idx + 1) ≠ slot s (idx + 6)
         [thm] inj: idx + 1 ≠ idx → slot s (idx + 1) ≠ slot s idx
         [thm] inj: idx + 7 ≠ idx + 1 → slot s (idx + 7) ≠ slot s (idx + 1)
+
 -/
 #guard_msgs in
 set_option grind.ematch.diagnostics true in
